Verif: file reorganization; add tsl capability mappings

theories/Verif/refine.v
@@ -3,340 +3,13 @@ From compcert Require Import Integers.
 From RecordUpdate Require Import RecordUpdate.
 From S3K.Barocq Require Import S3K_ShallowR.
 From S3K.ExecSem Require Import kstate cap ctx exec util config.
-From S3K.Verif Require Import repr barocq_aux tactics invariants.
-From S3K.BarocqComp Require Import Option Barray Intop Utils.
-From S3K.BarocqComp Require Import ShallowNotations.
-
-Set Implicit Arguments.
+From S3K.Verif Require Import repr safe_refine tactics refine_tactics bridge.
 
 (** * Refinement proofs *)
 
-(** ** Refinement with safe execution *)
-Section SafeRefine.
-
-(** A: abstract type, B: concrete type *)
-Variable A B : Type.
-
-(** R: Refinement mapping *)
-Variable R : A -> B -> Prop.
-
-(** Concrete code is safe while preserving refinement mapping. *)
-Definition safe_refine (a : A) (ob : option B) :=
-  exists b, ob = Some b /\ R a b.
-
-(** Concrete code is safe given that abstract code is safe, also maintaining
-refinement mapping. *)
-Definition safe_refine_opt (oa : option A) (ob : option B) :=
-  forall a, oa = Some a -> exists b, ob = Some b /\ R a b.
-
-Lemma safe_refine_opt_None : forall b, safe_refine_opt None b.
-Proof. done. Qed.
-
-Lemma safe_refine_opt_Some : forall a ob,
-  safe_refine a ob ->
-  safe_refine_opt (Some a) ob.
-Proof. unfold safe_refine_opt; intros; by inv H0. Qed.
-
-Lemma safe_refine_Some : forall a b,
-  R a b ->
-  safe_refine a (Some b).
-Proof. unfold safe_refine; intros; by exists b. Qed.
-
-End SafeRefine.
-
-(** ** Hints and tactics *)
-
-From Ltac2 Require Import Ltac2 Printf.
-Import tactics.Ltac2.
-
-Ltac2 Notation "lia" := ltac1:(lia).
-Ltac2 Notation "rep_lia" := ltac1:(rep_lia).
-
-Create HintDb s3k_unfold.
-(** Abstract helper functions to unfold *)
-Hint Unfold cap_get : s3k_unfold.
-Hint Unfold cap_owner_get : s3k_unfold.
-Hint Unfold cap_idx_valid : s3k_unfold.
-
-(** Barocq helper functions to unfold *)
-Hint Unfold Mon_valid_access : s3k_unfold.
-
-(** Hint database for backward reasoning about data correspondence between
-the abstract and concrete models. *)
-Create HintDb s3k_inv.
-
-Hint Resolve safe_refine_opt_None safe_refine_opt_Some safe_refine_Some : s3k_inv.
-Hint Resolve Rkstate_inv Rkstate_with_err_inv : s3k_inv.
-Hint Resolve Rmon_table_set Rmon_set_owner Rmon_set_cfree : s3k_inv.
-Hint Resolve Rmon_table_inv_Rkstate Rtsl_table_inv_Rkstate Rptable_inv_Rkstate : s3k_inv.
-Hint Resolve Rmon_Some_inv Rmon_None_inv : s3k_inv.
-Hint Resolve Rpid_opt_inv_Rmon : s3k_inv.
-
-Hint Extern 0 (Rpid_opt _ _) => reflexivity : s3k_inv.
-Hint Extern 0 => progress simpl : s3k_inv.
-(** Replace CapTable l with canonical form *)
-Hint Extern 0 (Rmon_table (CapTable _) _) =>
-  match! goal with | [ h : _ = CapTable _ |- _ ] => let h := Control.hyp h in rewrite <- $h end
-  : s3k_inv.
-Hint Extern 0 (_ <> O) => lia : s3k_inv.
-
-Opaque cap_set.
-
-(* Hint database for arithmetic reasoning. *)
-Create HintDb s3k_arith.
-
-Hint Unfold Rnat fun_hrel ofun_hrel int64_to_nat nat_to_int64 : s3k_arith.
-Hint Unfold Int64.add Int64.sub I64.of_u64 : s3k_arith.
-Hint Unfold err_success : s3k_arith.
-Hint Rewrite mon_sz_config : s3k_arith.
-Hint Rewrite Int64.repr_unsigned : s3k_arith.
-
-
-Ltac2 norm_length1 () :=
-  match! goal with
-  | [h : ?tb.[?i <- ?v] = Some ?tb' |- context[length ?tb'] ] =>
-    (* Barocq set doesn't change length. *)
-    let h := Control.hyp h in rewrite (bset_length $tb $i $v $h)
-  | [h : Rmon_table (CapTable ?ta) ?tb |- context[length ?tb]] =>
-    (* Normalize concrete table size into abstract table size. *)
-    let h := Control.hyp h in
-    rewrite <- (Rmon_table_len_same $h)
-  | [h : ctable_size (CapTable _) = _ |- _] =>
-    (* Normalize capability table size into configured number. *)
-    simpl in $h;
-    let h := Control.hyp h in
-    rewrite $h in *
-  end.
-
-Ltac2 Notation "norm_length" := repeat (norm_length1 ()).
-
-(* Introduce range constraints for variables involved in goal. *)
-Ltac2 forward_range1 () :=
-  match! goal with
-  | [ h : ?l !! ?ia = Some _ |- context[?ia]] =>
-    (* Range for valid index *)
-    let h := Control.hyp h in
-    extend (lookup_lt_Some _ _ _ $h)
-  | [ |- context[cfree ?c]] =>
-    (* Range for capability field cfree - always <= table size if wellformed *)
-    assert_if_new (cfree $c <= MON_SZ)%nat
-  | [ |- context[csize ?c]] =>
-    assert_if_new (csize $c <= MON_SZ)%nat
-  | [ |- context[(cfree ?ci + cfree ?cj)%nat]] =>
-      assert_if_new ($ci.(cfree) + $cj.(cfree) <= $ci.(csize))%nat
-  end.
-
-Ltac2 Notation "forward_range" :=
-  repeat (forward_range1 ()); norm_length.
-
-Ltac2 repr_elim1 () :=
-  match! goal with
-  | [|- context[Int64.unsigned (Int64.repr ?z)]] =>
-    rewrite Int64.unsigned_repr with (z:=$z) by rep_lia
-  | [ h : context[Int64.unsigned (Int64.repr ?z)] |- _ ] =>
-    rewrite Int64.unsigned_repr with (z:=$z) in $h by rep_lia
-  | [ |- Int64.repr _ = Int64.repr _] => f_equal
-  end.
-
-Ltac2 Notation "repr_elim" := repeat (repr_elim1 ()).
-
-(** Solve R correspondence using backward reasoning *)
-Ltac2 solve_corres () :=
-  eauto 20 with s3k_inv.
-
-(** Derive finer correspondence results from the hypotheses. *)
-Ltac2 forward_hyp_corres1 () :=
-  match! goal with
-  | [ h1 : Rpid_opt ?ova ?vb,
-      h2 : Rpid_opt ?ova' ?vb' |- context[?vb] ] =>
-      let h1 := Control.hyp h1 in
-      let h2 := Control.hyp h2 in
-      rewrite (Rpid_opt_inj $h1 $h2) in *
-  end.
-
-Ltac2 Notation "forward_hyp_corres" := repeat (forward_hyp_corres1 ()).
-
-Ltac2 solve_arith () :=
-  printf "Trying to solve arithmetic goal: %t" (Control.goal ());
-  forward_range;
-  forward_hyp_corres;
-  ltac1:(autounfold with s3k_arith in *);
-  ltac1:(autorewrite with s3k_arith in *);
-  repr_elim;
-  rep_lia.
-
-Hint Extern 100 (Rnat _ _) => solve_arith () : s3k_inv.
-Hint Extern 10 (err_success _ = _) => solve_arith () : s3k_inv.
-
-(* Try solve correspondence term t and return the hypothesis, may fail. *)
-Ltac2 get_or_solve_corres (t : constr) : constr :=
-  printf "solving corres %t" t;
-  let oh := List.find_opt (fun (_,_,ty) => Constr.equal t ty) (Control.hyps ()) in
-  match oh with
-  (* if in goal already *)
-  | Some (h_ident, _, _) => Control.hyp h_ident
-  (* try solve it if not *)
-  | None => 
-    let h := Fresh.in_goal @Hcorres in
-    lazy_match! t with
-    (* if arithmetic goal *)
-    | Rnat _ _ => assert $t as $h by solve_arith ()
-    | _ => assert $t as $h by solve_corres ()
-    end;
-    Control.hyp h
-  end.
-
-(** Case analysis on whether an abstract capability is physically deleted or not. *)
-Ltac2 forward_abstract_opt_cap (t : constr) :=
-  destruct $t eqn:? >
-  [ (* Some case, introduce capability field correspondence.results. *)
-    match! goal with
-    | [ hget : ?tlookup = Some ?va,
-        h : Rmon (Some ?va) ?vb |- _ ] =>
-      Control.assert_true (Constr.equal t tlookup);
-      let h := Control.hyp h in
-      let h' := @HRmon_corres in
-      pose proof (Rmon_Some_corres $h) as $h'; destruct_and? $h'
-    end
-  |
-    (* None case *)
-    (* Since in principle a system call should never touch a physically deleted
-       capability, we can be sure that the concrete level must return invalid
-       access. This is ensured since Int64.eq vb.(types_mon_t_owner) owner is alway
-       false in this case. *)
-    try (erewrite Rmon_None_corres by eauto)
-  ].
-
-(** Reason Barocq set success and simplify. *)
-Ltac2 forward_concrete_map_set () :=
-  match! goal with
-  | [ h: ?tb.[?ib] = Some _ |- context[?tb.[?ib <- ?v]]] =>
-    (* Rewrite the result of barocq set at the same index *)
-    let h := Control.hyp h in
-    let tb' := Fresh.in_goal @tb in
-    let htb' := Fresh.in_goal @Htb in
-    destruct (bget_Some_bset_Some $tb $ib $v $h) as [$tb' $htb'];
-    let htb' := Control.hyp htb' in
-    rewrite $htb'; simpl
-  end.
-
-Ltac2 forward_abstract_lookup_None (h : constr) :=
-  simpl;
-  lazy_match! goal with
-  | [ |- safe_refine_opt _ None _] =>
-    (* If abstract model fails, holds vacuously by safe_refine_opt. *)
-    auto with s3k_inv
-  | [ |- _] =>
-    (* Otherwise abstract model handles the lookup error, simplify in concrete. *)
-    lazy_match! (Constr.type h) with ?ta !! ?ia = None =>
-      match! goal with
-      | [ |- context[?tb.[USIZE.of_u64 ?ib]]] =>
-        let hi := get_or_solve_corres '(Rnat $ia $ib) in
-        trivial_erewrite ?(mon_lookup_None_len _ _ $h $hi); simpl
-      | [ |- _] => fail_with_msg "Found no correspondence for abstract lookup in concrete model."
-      end
-    end
-  end.
-
-Ltac2 forward_abstract_lookup_Some (h : constr) :=
-  lazy_match! (Constr.type h) with ?ta !! ?ia = Some ?va =>
-    match! goal with
-    | [ |- context[?tb.[USIZE.of_u64 ?ib]]] =>
-      (* Case for both index and table correspondence *)
-      (* Solve table correspondence *)
-      let htable := get_or_solve_corres '(Rmon_table (CapTable $ta) $tb) in
-      (* Solve index correspondence *)
-      let hi := get_or_solve_corres '(Rnat $ia $ib) in
-      (* 1. Rewrite the result of barocq get *)
-      let vb := Fresh.in_goal @vb in
-      let hvb := Fresh.in_goal @Hvb in
-      let hrmon := Fresh.in_goal @HRmon in
-      destruct (mon_get_Some_corres $htable $hi $h) as [$vb [$hvb $hrmon]];
-      let hvb:= Control.hyp hvb in
-      trivial_erewrite ?($hvb), ?(mon_lookup_Some_len _ _ $h $hi); simpl;
-      (* 2. Destruct abstract optional capability *)
-      printf "Case analysis on whether abstract capability is physically deleted or not ";
-      Control.enter (fun _ => forward_abstract_opt_cap va);
-      (* 3. Forward barocq set at the same index *)
-      try (forward_concrete_map_set ())
-    | [ |- context[?tb.[USIZE.of_u64 ?ib]]] =>
-      (* Case for only index correspondence. Since barocq has in-place-update semantic,
-         table may be different. Can still simplify for safe execution. *)
-      printf "trying to just solve hi: %t" '(Rnat $ia $ib); 
-      let hi := get_or_solve_corres '(Rnat $ia $ib) in
-      (* 1. Barocq get safe *)
-      let hlen := Fresh.in_goal @Hlen in
-      (*assert (length $ta = length $tb) as $hlen by solve_length ();*)
-      assert (length $ta = length $tb) as $hlen by (norm_length; congruence);
-      let hlen := Control.hyp hlen in
-      let vb := Fresh.in_goal @vb in
-      let hvb := Fresh.in_goal @Hvb in
-      destruct (lookup_Some_bget_safe $ta $tb $h $hi $hlen) as [$vb $hvb];
-      let hvb := Control.hyp hvb in
-      rewrite ?($hvb); simpl;
-      (* 2. Barocq set safe *)
-      try (forward_concrete_map_set ())
-    end
-  end.
-
-Ltac2 forward_abstract_lookup (h : constr) :=
-  lazy_match! (Constr.type h) with
-  | _ !! _ = Some _ => forward_abstract_lookup_Some h
-  | _ !! _ = None => forward_abstract_lookup_None h
-  end.
-
-(** Solve concrete condition. *)
-Ltac2 solve_concrete_cond () :=
-  printf "Trying to solve concrete condition: %t" (Control.goal ());
-  (* normalize hypotheses *)
-  destruct_and?; destruct_or?;
-  forward_hyp_corres;
-  (* normalize goal *)
-  ltac1:(autounfold with s3k_arith in *);
-  ltac1:(norm_bool_cmp);
-  repr_elim;
-  rep_lia.
-
-(** Find head concrete condition and try simplifying it. *)
-Ltac2 forward_concrete_cond () :=
-  match! goal with
-  | [ |- _ _ _ (if ?b then _ else _)] =>
-    (* Try simplify the if branch *)
-    let hcond := Fresh.in_goal @Hcond in
-    first [
-      assert ($b = true) as $hcond by solve_concrete_cond () |
-      assert ($b = false) as $hcond by solve_concrete_cond () ];
-    let hcond := Control.hyp hcond in
-    rewrite! $hcond; simpl
-  | [ |- _ ] => printf "Failed to solve any concrete condition."
-  end.
-  
-(** Find decision in abstract model, do case analysis and try simplifying and
-synchronizing the concrete model. *)
-Ltac2 forward_abstract () :=
-  match! goal with
-  | [ |- context[match ?t with  _ => _ end ] ] =>
-      first [
-        lazy_match! (Constr.type t) with
-        (* Destruct cap table of single construtor CapTable *)
-        | mon_table_t => destruct $t eqn:?; printf "Getting rid of CapTable"
-        | cap_table_t _  => destruct $t eqn:?; printf "Getting rid of CapTable"
-        end |
-        lazy_match! t with
-        |  ?l !! ?ia =>
-          (* Destruct result of abstract lookup *)
-            let h := Fresh.in_goal @Hlookup in
-            printf "Case analysis on capability table lookup";
-            destruct $t eqn:$h; Control.enter (fun () => forward_abstract_lookup (Control.hyp h))
-        | decide ?p =>
-          (* Destruct abstract decision, also try derive facts for concrete level  *)
-          ltac1:(case_decide); Control.enter (fun () => forward_concrete_cond () )
-        end
-      ]
-  end.
-
-
 (** ** Refinement proofs for capability operations. *)
+
+Ltac prepare := intros; autounfold with s3k_unfold.
 
 Section S3KRefine.
 
@@ -373,11 +46,9 @@ Theorem mon_delele_safe_refine :
   Rnat ia ib ->
   safe_refine Rkstate_with_err (exec_mon_delete ka ownera ia) (Mon_delete kb ownerb ib).
 Proof.
-  intros.
   unfold exec_mon_delete, Mon_delete.
-  ltac1:(autounfold with s3k_unfold).
-  repeat (forward_abstract ()).
-  all: solve_corres ().
+  prepare.
+  repeat forward_abstract; solve_corres.
 Qed.
 
 Theorem mon_transfer_safe_refine :
@@ -388,11 +59,9 @@ Theorem mon_transfer_safe_refine :
   Rpid_opt (Some new_ownera) new_ownerb ->
   safe_refine Rkstate_with_err (exec_mon_transfer ka ownera ia new_ownera) (Mon_transfer kb ownerb ib new_ownerb).
 Proof.
-  intros.
   unfold exec_mon_transfer, Mon_transfer.
-  ltac1:(autounfold with s3k_unfold).
-  repeat (forward_abstract ()).
-  all: solve_corres ().
+  prepare.
+  repeat forward_abstract; solve_corres.
 Qed.
 
 Theorem mon_derive_safe_refine :
@@ -403,14 +72,10 @@ Theorem mon_derive_safe_refine :
   Rnat csizea csizeb ->
   safe_refine_opt Rkstate_with_err (exec_mon_derive ka ownera ia csizea) (Mon_derive kb ownerb ib ownerb csizeb).
 Proof.
-  intros. 
   unfold exec_mon_derive, Mon_derive.
-  ltac1:(autounfold with s3k_unfold).
-  repeat (forward_abstract ()).
-  all: solve_corres ().
+  prepare.
+  repeat forward_abstract; solve_corres.
 Qed.
-
-From S3K.Verif Require Import bridge.
 
 Theorem mon_revoke_safe_refine :
   forall ownera ownerb ia ib,
@@ -419,11 +84,9 @@ Theorem mon_revoke_safe_refine :
   Rnat ia ib ->
   safe_refine_opt Rkstate_with_err (exec_mon_revoke' ka ownera ia) (Mon_revoke kb ownerb ib).
 Proof.
-  intros.
   unfold exec_mon_revoke', Mon_revoke, Mon_revoke_once.
-  ltac1:(autounfold with s3k_unfold).
-  repeat (forward_abstract ()).
-  all: solve_corres ().
+  prepare.
+  repeat forward_abstract; solve_corres.
 Qed.
 
 End S3KRefine.
