theories/Verif/safe_refine.v
@@ -1,0 +1,37 @@
+From stdpp Require Import prelude.
+
+Set Implicit Arguments.
+
+(** * Refinement with safe execution *)
+Section SafeRefine.
+
+(** A: abstract type, B: concrete type *)
+Variable A B : Type.
+
+(** R: Refinement mapping *)
+Variable R : A -> B -> Prop.
+
+(** Concrete code is safe while preserving refinement mapping. *)
+Definition safe_refine (a : A) (ob : option B) :=
+  exists b, ob = Some b /\ R a b.
+
+(** Concrete code is safe given that abstract code is safe, also maintaining
+refinement mapping. *)
+Definition safe_refine_opt (oa : option A) (ob : option B) :=
+  forall a, oa = Some a -> exists b, ob = Some b /\ R a b.
+
+Lemma safe_refine_opt_None : forall b, safe_refine_opt None b.
+Proof. done. Qed.
+
+Lemma safe_refine_opt_Some : forall a ob,
+  safe_refine a ob ->
+  safe_refine_opt (Some a) ob.
+Proof. unfold safe_refine_opt; intros; by inv H0. Qed.
+
+Lemma safe_refine_Some : forall a b,
+  R a b ->
+  safe_refine a (Some b).
+Proof. unfold safe_refine; intros; by exists b. Qed.
+
+End SafeRefine.
+
